# 괄호변환
# https://programmers.co.kr/learn/courses/30/lessons/60058

## solution 1
```python
def convert_balance(p):
    for i in range(0, len(p), 2):
        u = p[0: i+2]
        if u.count('(') == u.count(')'):
            v = p[i+2:]
            break
    return u, v

def convert_u(u):
    temp = ''
    for paren in u[1:-1]:
        if paren == '(':
            temp+=')'
        else:
            temp+='('
    return temp

def change_parenthesis(p):
    if not p:
        return p
    
    u, v = convert_balance(p)
    
    if check_paraenthesis(u):
        return u + change_parenthesis(v)
    else:
        u_temp = convert_u(u)
        return '(' + change_parenthesis(v) + ')' + u_temp

        
def check_paraenthesis(s):
    stack = []

    for v in s:
        if v == '(':
            stack.append('(')
        else:
            if stack:
                stack.pop()
            else:
                return False
    return stack == []

def solution(p):
    # p = '))(()())(('
    if check_paraenthesis(p):
        return p
    
    k = change_parenthesis(p)
    # print(k)
    return k
``` 

## solution 2 
```python
def split_u_v(str_):
    for index in range(1, len(str_)+1):
        if str_[:index].count('(') == str_[:index].count(')'):
            return str_[:index], str_[index:]

def check_u(u):
    stack = []
    for char in u:
        if not stack:
            stack.append(char)
        else:
            if char == ')' and stack [-1] == '(':
                stack.pop()
            elif char == '(':
                stack.append(char)
    return not stack

def get_balance(u, v):
    result = '(' + conversion(v) + ')' 
    for i in u[1:-1]:
        if i == '(':
            result += ')'
        elif i == ')':
            result += '('
    return result

def conversion(p):
    if not p:
        return p
    u, v = split_u_v(p)
    if check_u(u):
        return u + conversion(v)
    else:
        return get_balance(u, v)
    
def solution(p):
    answer = conversion(p)
    return answer
``` 


